Try to proof formula soundness (but the termination assumption is INCONSISTENT\!)

HML_Strategies_Game.thy
@@ -13,8 +13,13 @@ fixes
   strat :: \<open>('s, 'a) c_set_game_node posstrategy\<close> and
   winning_dist :: \<open>('s, 'a) c_set_game_node \<Rightarrow> nat\<close>
 assumes
-  winning_dist_decreasing: \<open>winning_dist (strat pos) < winning_dist pos\<close>
+  \<comment>\<open>This assumption seems to create an inconsistency.... :/ Will have to restrict it to non-immediately attacker-won positions (?)\<close>
+  winning_dist_decreasing: \<open>\<And>pos. winning_dist (strat pos) < winning_dist pos\<close>
 begin
+
+lemma INCONSISTENCY:
+  False using winning_dist_decreasing wf_measure[of winning_dist] wf_def
+  by (meson UNIV_I in_measure wf_eq_minimal)
 
 text \<open>This construction of attacker formulas from a game only works if \<open>strat\<close> is a (non-cyclic)
   attacker strategy. (If it's winning and sound, the constructed formula should be distinguishing.)\<close>
@@ -23,9 +28,9 @@ function attack_formula :: \<open>('s, 'a) c_set_game_node \<Rightarrow> ('a,'s)
   \<open>attack_formula (AttackerNode p Q) =
     attack_formula (strat ((AttackerNode p Q)))\<close>
 | \<open>attack_formula (DefenderSimNode a p Q) =
-    (HML_poss a (attack_formula (AttackerNode p Q)))\<close>
+    \<langle>\<tau>\<rangle>\<langle>a\<rangle>(attack_formula (AttackerNode p (dsuccs a Q)))\<close>
 | \<open>attack_formula (DefenderSwapNode p Q) =
-    (HML_weaknor Q (\<lambda>q. (attack_formula (AttackerNode q {p}))))\<close>
+    (HML_weaknor (weak_tau_succs Q) (\<lambda>q. (attack_formula (AttackerNode q {p}))))\<close>
   using c_set_game_defender_node.cases
   by (auto, blast)
 
@@ -34,6 +39,141 @@ termination attack_formula
     wf_measure[of winning_dist]
   unfolding wf_def
   by auto
+
+lemma attack_options: 
+  assumes
+    \<open>player1_winning_strategy (strategy_from_positional strat) (AttackerNode p Q)\<close>
+    \<open>sound_1strategy (strategy_from_positional strat) (AttackerNode p Q)\<close>
+  shows
+    \<open>(\<exists>a p'. attack_formula (AttackerNode p Q) = \<langle>\<tau>\<rangle>\<langle>a\<rangle>(attack_formula (AttackerNode p' (dsuccs a Q))))
+    \<or> (\<exists>p'. attack_formula (AttackerNode p Q) = (HML_weaknor (weak_tau_succs Q) (\<lambda>q. (attack_formula (AttackerNode q {p'})))))\<close>
+proof -
+  have \<open>[AttackerNode p Q] \<in> plays_for_1strategy (strategy_from_positional strat) (AttackerNode p Q)\<close>
+    using plays_for_1strategy.init by auto
+  with assms(1) have unstuck:
+    \<open>\<exists>p'. c_set_game_moves (AttackerNode p Q) p'\<close>
+    unfolding player1_winning_strategy_def player0_wins_immediately_def by fastforce
+  with assms(2) have \<open>c_set_game_moves (AttackerNode p Q) (strat (AttackerNode p Q))\<close>
+    unfolding sound_1strategy_def strategy_from_positional_def
+    using plays_for_1strategy.init by fastforce
+  hence \<open>(\<exists>a p'. p =\<rhd>a p' \<and> \<not> tau a \<and> strat (AttackerNode p Q) = (DefenderSimNode a p' Q))
+    \<or> (\<exists>p'. p \<Rightarrow>^\<tau> p' \<and> strat (AttackerNode p Q) = (DefenderSwapNode p' Q))\<close>
+    using c_set_game_defender_node.elims(1) c_set_game_moves_no_step(5) simulation_challenge swap_challenge
+    by (smt (verit))
+  hence  \<open>(\<exists>a p'. attack_formula (AttackerNode p Q) = (attack_formula (DefenderSimNode a p' Q)))
+    \<or> (\<exists>p'. attack_formula (AttackerNode p Q) = (attack_formula (DefenderSwapNode p' Q)))\<close>
+    by auto
+  thus ?thesis by simp
+qed
+
+thm attack_formula.induct
+
+lemma Apparently_something_is_inconsistent:
+  shows False using attack_formula.induct by blast
+
+lemma distinction_soundness:
+  fixes p Q p0 Q0
+  defines
+    \<open>pQ == AttackerNode p Q\<close>
+  defines
+    \<open>\<phi> == attack_formula pQ\<close>
+  assumes
+    \<open>\<exists>rest. pQ # rest \<in> plays_for_1strategy (strategy_from_positional strat) (AttackerNode p0 Q0)\<close>
+    \<open>player1_winning_strategy (strategy_from_positional strat) pQ\<close>
+    \<open>sound_1strategy (strategy_from_positional strat) pQ\<close>
+  shows
+    \<open>p \<Turnstile> \<phi> \<and> (\<forall>q\<in>Q. \<not> q \<Turnstile> \<phi>)\<close>
+  using assms(3,4,5) unfolding assms(1,2)
+  by (induct arbitrary: p Q rule: attack_formula.induct[of _ \<open>(AttackerNode p Q)\<close>], auto)
+
+lemma distinction_soundness:
+  fixes p Q rest p0 Q0
+  defines
+    \<open>pQ == AttackerNode p Q\<close>
+  defines
+    \<open>\<phi> == attack_formula pQ\<close>
+  assumes
+    \<open>\<exists>rest. pQ # rest \<in> plays_for_1strategy (strategy_from_positional strat) (AttackerNode p0 Q0)\<close>
+    \<open>player1_winning_strategy (strategy_from_positional strat) pQ\<close>
+    \<open>sound_1strategy (strategy_from_positional strat) pQ\<close>
+  shows
+    \<open>p \<Turnstile> \<phi> \<and> (\<forall>q\<in>Q. \<not> q \<Turnstile> \<phi>)\<close>
+  using assms(1,3,4,5) unfolding \<open>\<phi> == attack_formula pQ\<close>
+
+
+  case (1 p' Q')
+  then show ?case sorry
+next
+  case (2 a p Q)
+  then show ?case sorry
+next
+  case (3 p Q)
+  then show ?case sorry
+qed
+  case (1 p' Q')
+  then show ?case sorry
+next
+  case (2 a p' Q')
+  then show ?case by auto
+next
+  case (3 p' Q')
+  then show ?case by auto
+qed
+  case (1)
+  then show ?case sorry
+next
+  case 2
+  then show ?case sorry
+next
+  case 3
+  then show ?case sorry
+qed
+  case (1 p' Q')
+  then show ?case sorry
+next
+  case (2 a p' Q')
+  then show ?case sorry
+next
+  case (3 p' Q')
+  then show ?case sorry
+qed
+
+
+
+  case HML_true
+  hence \<open>False\<close> using attack_options HML_weaknor_def HML_formula.distinct(5)
+    by metis
+  then show ?case ..
+next
+  case (HML_conj Q F)
+  hence \<open>False\<close> using attack_options HML_weaknor_def HML_formula.distinct(9)
+    by metis
+  then show ?case ..
+next
+  case (HML_neg \<phi>)
+  hence \<open>False\<close> using attack_options HML_weaknor_def HML_formula.distinct(11)
+    by metis
+  then show ?case ..
+next
+  case (HML_poss t \<phi>)
+  hence \<open>(\<exists>a p'. attack_formula (AttackerNode p Q) = \<langle>\<tau>\<rangle>\<langle>a\<rangle>(attack_formula (AttackerNode p' (dsuccs a Q))))
+    \<or> (\<exists>p'. attack_formula (AttackerNode p Q) = \<langle>\<tau>\<rangle>(AND (weak_tau_succs Q) (\<lambda>q. HML_neg (attack_formula (AttackerNode q {p'})))))\<close>
+    using attack_options[of p Q] unfolding HML_weaknor_def by blast
+  hence
+    \<open>t = \<tau>\<close>
+    \<open>(\<exists>a p'. \<phi> = \<langle>a\<rangle>(attack_formula (AttackerNode p' (dsuccs a Q))))
+    \<or> (\<exists>p'. \<phi> = (AND (weak_tau_succs Q) (\<lambda>q. HML_neg (attack_formula (AttackerNode q {p'})))))\<close>
+    using \<open>(\<langle>t\<rangle>\<phi>) = attack_formula (AttackerNode p Q)\<close> by auto
+  from this(2) show ?case unfolding \<open>t = \<tau>\<close>
+  proof (rule disjE)
+    assume \<open>\<exists>a p'. \<phi> = \<langle>a\<rangle>attack_formula (AttackerNode p' (dsuccs a Q))\<close>
+    then obtain a p' where phi_def: \<open>\<phi> = \<langle>a\<rangle>attack_formula (AttackerNode p' (dsuccs a Q))\<close> by blast
+    have \<open>player1_winning_strategy (strategy_from_positional strat) (AttackerNode p' (dsuccs a Q))\<close>
+        \<open>sound_1strategy (strategy_from_positional strat) (AttackerNode p' (dsuccs a Q))\<close> sorry
+    with HML_poss(1) phi_def have \<open>p' \<Turnstile> \<phi> \<and> (\<forall>q\<in>(dsuccs a Q). \<not> q \<Turnstile> \<phi>)\<close>
+    show \<open>(p \<Turnstile> (\<langle>\<tau>\<rangle>\<phi>)) \<and> (\<forall>q\<in>Q. \<not> (q \<Turnstile> (\<langle>\<tau>\<rangle>\<phi>)))\<close> sorry
+  qed
+qed
 
 end
 end
